\documentclass{article}
\usepackage{CJK}
\usepackage{amsmath,amssymb}
\usepackage{fancyhdr}  


\begin{document}
\begin{CJK*}{GBK}{song}

\pagestyle{fancy}  
\fancyhead{} % clear all fields  
\fancyhead[R]{Group Theory}  
\fancyhead[L]{Chenxi Gu\\ 2017311017} 
\renewcommand{\headrulewidth}{0.4pt}  
\renewcommand{\footrulewidth}{0.4pt} 



\title {homework 2}
\author{Chenxi Gu\\2017311017}

\date{\today}

\maketitle

\section{2.2}
$A(g_a)$ is a representation.
\begin{equation}
A(g_1)A(g_2)=A(g_1g_2)
\end{equation}

So we can get :
\begin{equation}
A^T(g_1)^{-1}A^T(g_2)^{-1}=[[A(g_1)A(g_2)]^T]^{-1}=A^T(g_1g_2)^{-1}
\end{equation}





\begin{equation}
A^{\dagger}(g_1)^{-1}A^{\dagger}(g_2)^{-1}=[[A(g_1)A(g_2)]^{\dagger}]^{-1}=A^{\dagger}(g_1g_2)^{-1}
\end{equation}

$A^T(g_a)^{-1},A^{\dagger}(g_a)^{-1}$ are also representation.\\


$A^T(g_a),A^{\dagger}(g_a)$ are not representation,but Abel group.
if $A(g_a)$ is a Unitary representation:
\begin{equation}
\begin{aligned}
&A^{\dagger}(g)=A(g^{-1})\\
&A^{T\dagger}(g)^{-1}=A^T(g)\\
&A^{\dagger \dagger}(g)^{-1}=A(g)^{-1}
\end{aligned}
\end{equation}
So $A^T(g)^{-1},A^{\dagger}(g)^{-1}$ are unitary representation.It is esay to prove they are irreducible representation.

\section{2.3}
It is easy to find the matrix commute with all elements in group $A(g)$:
\begin{equation}
[A(g_a),\sum_CA(g_b)]=0
\end{equation} 
Using shur lemma :
\begin{equation}
\sum_CA(g_b)=\lambda E
\end{equation}

\section{2.7}
We choose natural basic :
\begin{equation}
e=
\begin{pmatrix}
     1 \\
     0 \\
     0 \\
     0 \\
\end{pmatrix}\quad
a=
\begin{pmatrix}
     0 \\
     1 \\
     0 \\
     0 \\
\end{pmatrix}\quad
a^2=
\begin{pmatrix}
     0 \\
     0 \\
     1 \\
     0 \\
\end{pmatrix}\quad
a^3=
\begin{pmatrix}
     0 \\
     0 \\
     0 \\
     1 \\
\end{pmatrix}
\end{equation}
So we can get the left representation:
\begin{equation}
L(e)=
\begin{pmatrix}
     1  &  0  &  0  &  0\\
     0  &  1  &  0  &  0\\
     0  &  0  &  1  &  0\\
     0  &  0  &  0  &  1\\
\end{pmatrix}\quad
L(a)=
\begin{pmatrix}
     0  &  0  &  0  &  1\\
     1  &  0  &  0  &  0\\
     0  &  1  &  0  &  0\\
     0  &  0  &  1  &  0\\
\end{pmatrix}
\end{equation}
The right presentation:
\begin{equation}
R(e)=
\begin{pmatrix}
     1  &  0  &  0  &  0\\
     0  &  1  &  0  &  0\\
     0  &  0  &  1  &  0\\
     0  &  0  &  0  &  1\\
\end{pmatrix}\quad
R(a)=
\begin{pmatrix}
     0  &  1  &  0  &  0\\
     0  &  0  &  1  &  0\\
     0  &  0  &  0  &  1\\
     1  &  0  &  0  &  0\\
\end{pmatrix}
\end{equation}





\section{2.8}


































\end{CJK*}
\end{document}

