

\documentclass{article}
\usepackage{CJK}
\usepackage{amsmath,amssymb}
\usepackage{fancyhdr}  


\begin{document}
\begin{CJK*}{GBK}{song}

\pagestyle{fancy}  
\fancyhead{} % clear all fields  
\fancyhead[R]{Data Analysis}  
\fancyhead[L]{Chenxi Gu\\ 2017311017} 
\renewcommand{\headrulewidth}{0.4pt}  
\renewcommand{\footrulewidth}{0.4pt} 



\title {chapter 2}
\author{Chenxi Gu\\2017311017}

\date{\today}

\maketitle
\section{2.1}
\begin{equation}
\begin{aligned}
\sigma^2_k&=\sum_{i,j=1}^MV_{ij}\\
&=\sum_{i,j=1}^M(\delta_{ij}n_{tot}p_i(1-p_i)+(\delta_{ij}-1)p_ip_jn_{tot})\\
&=\sum_{i=1}^M(n_{tot}p_i(1-p_i)-p_i(p_0-p_i)n_{tot})\\
&=n_{tot}(p_0-p_0^2)\\
\end{aligned}
\end{equation}
While $p_0=\sum_{i=1}^Mp_i$


\section{2.2}
\begin{equation}
\begin{aligned}
&E[\frac{1}{x}]=\int^{\beta}_{\alpha}\frac{In(\beta)-In(\alpha)}{\beta-\alpha}=In(2)\\
&\frac{1}{E[x]}=\frac{2}{\beta+\alpha}=\frac{2}{3}
\end{aligned}
\end{equation}

\section{2.3}
(a)
\begin{equation}
F(x)=\int^x_0f(x)dx=1-e^{-\frac{x}{\xi}}
\end{equation}
(b)
\begin{equation}
P(x\le x^{'})=F(x^{'})=1-e^{-\frac{x^{'}}{\xi}}
\end{equation}
\begin{equation}
P(x\le x^{'}+x_0|x\ge x_0)=\frac{P(x_0\le x\le x^{'}+x_0)}{P(x\ge x_0)}=\frac{e^{-\frac{x_0}{\xi}}-e^{-\frac{x_0+x^{'}}{\xi}}}{e^{-\frac{x_0}{\xi}}}=1-e^{-\frac{x^{'}}{\xi}}
\end{equation}
(c)
\begin{equation}
P(Decay In Detector|Enter Detector)=P(t\le t_0)
\end{equation}
So the time before the detector doesn't affect the lifetime.

\section{2.4}
(a)It is easy to say $\phi(x)$ is a Gaussian distribution.
\begin{equation}
\begin{aligned}
&E[x]=E[\frac{y-\mu}{\sigma}]=\frac{E[y]-\mu}{\sigma}=0\\
&V[x]=V[\frac{y-\mu}{\sigma}]=\frac{V[y]}{\sigma^2}=1
\end{aligned}
\end{equation}
(b)
\begin{equation}
F(y)=\int\frac{1}{\sqrt{2\pi}\sigma}e^{-\frac{(y-\mu)^2}{2\sigma^2}}dy
\end{equation}
\begin{equation}
\Phi(x)=\int\frac{1}{\sqrt{2\pi}}e^{-\frac{x^2}{2}}dx
\end{equation}
We could do variable substitution $x=\frac{y=\mu}{\sigma}$, equation(7),(8) are same.

\section{2.5}
(a)
\begin{equation}
g(y)dy=f(x)dx
\end{equation}
\begin{equation}
f(x)=g(y)\frac{dy}{dx}=\frac{1}{\sqrt{2\pi}\sigma x}e^{-\frac{(y-\mu)^2}{2\sigma^2}}=\frac{1}{\sqrt{2\pi}\sigma x}e^{-\frac{(In(x)-\mu)^2}{2\sigma^2}}
\end{equation}

(b)
\begin{equation}
\begin{aligned}
E[x]&=\int\frac{1}{\sqrt{2\pi}\sigma}e^{-\frac{(In(x)-\mu)^2}{2\sigma^2}}dx\\
&=\int\frac{1}{\sqrt{2\pi}\sigma}e^{-\frac{(y-\mu)^2}{2\sigma^2}}e^ydy\\
&=\int\frac{1}{\sqrt{2\pi}\sigma}e^{-\frac{(y-\mu-\sigma^2)^2}{2\sigma^2}}e^{\mu+\sigma^2/2}dy\\
&=e^{\mu+\sigma^2/2}
\end{aligned}
\end{equation}

\begin{equation}
\begin{aligned}
V[x]&=\int(x-E[x])^2f(x)dx\\
&=\int x^2f(x)dx-E[x]^2\\
&=\int\frac{1}{\sqrt{2\pi}\sigma}e^{-\frac{(y-\mu-2\sigma^2)^2}{2\sigma^2}}e^{2\mu+2\sigma^2}dy-e^{2\mu+\sigma^2}\\
&=e^{2\mu+2\sigma^2}-e^{2\mu+\sigma^2}
\end{aligned}
\end{equation}
(c)
According to error transfer formula:
\begin{equation}
\sigma_x^2=e^{2\mu}\sigma^2
\end{equation}
When $\sigma^2\ll1$ and $\sigma^2\ll\mu$, the formula is great.



\section{2.6}
\begin{equation}
\begin{aligned}
F_{\chi^2}(z;n)&=\int_0^z\frac{1}{2^{n/2}\Gamma(n/2)}z^{n/2-1}e^{-z/2}dz\\
&let \quad x=z/2\\
&=\int_0^{\frac{z}{2}}\frac{1}{\Gamma(n/2)}x^{n/2-1}e^{-x}dx\\
&=P(\frac{z}{2},\frac{n}{2})
\end{aligned}
\end{equation}






\end{CJK*}
\end{document}
